updates

Veritas.MultiSet.fst
@@ -8,3 +8,10 @@ let mem (#a:eqtype) (x:a) (s:mset a): Tot nat = admit()
 
 (* empty set *)
 let empty (#a:eqtype): Tot (mset a) = admit()
+
+let lemma_empty_implies_notmem (#a: eqtype) (s: mset a) (x: a):
+  Lemma (requires (is_empty s))
+        (ensures (~ (contains s x))) = admit()
+
+(* construct a multiset given a sequence *)
+let seq2mset (#a:eqtype) (s: seq a): Tot (mset a) = admit()
