Veritas.MultiSet.fsti
@@ -1,5 +1,7 @@
 module Veritas.MultiSet
 
+open FStar.Seq
+
 val mset (a:eqtype): Type0
 
 val equal (#a:eqtype) (s1:mset a) (s2:mset a): Tot bool
@@ -10,4 +12,16 @@ val mem (#a:eqtype) (x:a) (s:mset a): Tot nat
 (* empty set *)
 val empty (#a:eqtype): Tot (mset a)
 
+(* does a multiset contain an element x *)
+let contains (#a:eqtype) (s:mset a) (x:a) = mem x s = 0 
 
+let is_empty (#a:eqtype) (s:mset a) = 
+  equal s empty
+
+(* the empty set does not contain anything *)
+val lemma_empty_implies_notmem (#a: eqtype) (s: mset a) (x: a):
+  Lemma (requires (is_empty s))
+        (ensures (~ (contains s x)))
+
+(* construct a multiset given a sequence *)
+val seq2mset (#a:eqtype) (s: seq a): Tot (mset a)
