Veritas.Verifier.Defs.fst
@@ -3,3 +3,5 @@ module Veritas.Verifier.Defs
 let hashfn (m:merkle_payload): hash_value = admit()
 
 let empty_hash_value = zero_vec 
+
+let ms_hashfn_upd (e:ms_hashfn_dom) (h:ms_hash_value): ms_hash_value = admit()
